\documentclass[11pt]{article}
\usepackage{enumitem}
\usepackage{amsmath,amsthm,amssymb}

\begin{document}
\title{Homework 7}
\author{Brennen Green}
\maketitle


\begin{enumerate}
    \item \begin{enumerate}
        \item 2, 12, 72, 432, 2592, 15552
        \item 2, 4, 16, 256, 65536, 4294967296
        \item 1, 2, 5, 11, 26, 59
        \item 1, 1, 6, 27, 204, 1695
        \item 1, 2, 0, 1, 3, 3
    \end{enumerate}
    \item \begin{enumerate}
        \item -3(0) + 4(0) = 0 = $a_n$
        \item -3(1) + 4(1) = 1 = $a_n$
        \item $-3(-4^{n-1}) + 4(-4^{n-2}) = -3(-4)(-4^{n-2}) + 4(-4^{n-2})$
        $ = (-4)^{n-2}*(-4)^2 = -4^n$
        \item $ -3(2(-4)^{n-1}+3)+4(2(-4)^{n-2}+3) $\newline
        $ = -6(-4)^{n-1}-9+4(2(-4)^{n-2}+3)$\newline
        $ = (-4)^{n-2}(-6*(-4)+8)+3 $\newline
        $ = (-4)^{n-2}(16)(2)+3 $\newline
        $ = 2(-4)^n + 3 = a_n $
    \end{enumerate}
    \item \begin{enumerate}
        \item $ a_n = a_{n-1}*1.09 \; a_0 = 1000$
        \item $ 1.09^n * 1000 $
        \item $ \$5,529,041 $
    \end{enumerate}
    \item \begin{enumerate}
        \item $a_n = a_{n-1} + a_{n-2} + 2^{n-2}$
        \item $a_0 = 0 \; a_1=0 \;$
        \item $a_7 = a_6 + a_5 + 2^5 = 43 + 19 + 32 = 94$
    \end{enumerate}
    \newpage
    \item \begin{enumerate}
        \item Linear Homogenous Relationship with degree of 2
        \item Not Homogenous
        \item Not Linear
        \item Linear Homogenous Relationship with degree of 3
        \item Not Linear
        \item Not Homogenous
        \item Linear Homogenous Relationship with degree of 7
    \end{enumerate}
    \item \begin{enumerate}
        \item $P_n = 1.2P_{n-1} + 0.45P_{n-2} \; P_0 = \$100,000 \; P_1 = \$120,000$
        \item $P_n = (\frac{250000}{3})*(\frac{3}{2})^n + (50000)*(-\frac{3}{10})^n$
    \end{enumerate}
    \item $ a_n = 5 + 3(-2)^n - 3^n $
    \item $ a_n = \alpha_1 * (1)^n + \alpha_2 * (-2)^n + \alpha_3 * (3)^n + \alpha_4 * (-4)^n $ 
    \item \begin{align*}
        & f(64) = f(32) + 2 \\
        & = f(16) + 2 + 2 \\
        & = f(8) + 2 + 2 + 2 \\
        & = f(4) + 2 + 2 + 2 + 2 \\
        & = f(2) + 2 + 2 + 2 + 2 + 2 \\
        & = f(1) + 2 + 2 + 2 + 2 + 2 + 2 \\
        & = 2 + 12 = 14 \text{ comparisons}\\
    \end{align*}
    \item \begin{enumerate}
        \item $f(3) = f(1) + 1 = 1+1 = 2$
        \item $f(27) = f(9) + 1 = f(3) + 1 + 1 = f(1) + 1 + 1 + 1 = 4$
        \item $f(729) = f(243) + 1 = f(81) + 2 = f(27) + 3 = f(9) + 4$\newline
        $=f(3) + 5 = f(1) + 6 = 7 $
    \end{enumerate}
    \item \begin{align*}
        & f(n) = 2f(\frac{n}{3}) + 4 \\
        & f(3^k) = 2f(3^{k-1}) + 4 \\
        & \dots \\
        & = 2^k * f(1) + 4(2^k - 1) \\
        & = 2^k + 4(2^k - 1) \\
        & = 2^k + 2^{k+2} - 4 \\
    \end{align*}
    \item \begin{proof}
        \begin{align*}
            & f(n) = C_1 * n^d + C_2 * n^{\log_b{a}} \\
            & C_1 = \frac{b^d * c}{b^d - 1} \; C_2 = \frac{b^d * c}{a - b^d} \\
            & a = 5 \; b = 4 \; c = 6 \; d = 1 \; \text{(Divide and Conquer Recurrence Relation)}\\
            & C_1 = -24 \; C_2 = 25 \\
            & f(n) = -24n + 25n^{\log_4{5}} \\
            & f(4^k) = -24(4^k) + 25(4^k)^{\log_4{5}} \\
            & = 3 * 2^{2k+3} + 25(4^k)^{\log_4{5}} \\
            & = 3 * 2^{2k+3} + 5^{k+2} \qedhere
        \end{align*}
    \end{proof}
    \item \begin{enumerate}
        \item 1024
        \item 11
        \item 66
        \item 292,864
        \item 20,412
    \end{enumerate}
    \item $ a_k = 3*a_{k-1} + 2 = 2*3^k - 1  $
    \item \begin{enumerate}
        \item 30
        \item 29
        \item 24
        \item 18
    \end{enumerate}
    \item $(650,000+1,250,000) - 1,450,000 = 450,000$
    \item \begin{enumerate}
        \item 10,000
        \item 11,100
        \item 11,095
    \end{enumerate}
    \item 68 of the integers not exceeding 100 are divisible by 5 or 7
\end{enumerate}

\end{document}

